1st tentative for tableaux

LRrule/schensted.v
@@ -1,6 +1,8 @@
 Require Import ssreflect ssrbool ssrfun ssrnat eqtype fintype choice seq.
-
 Require Import subseq.
+
+Set Implicit Arguments.
+Unset Strict Implicit.
 
 Section Rows.
 
@@ -87,79 +89,82 @@ Section Schensted.
   Implicit Type l : nat.
   Implicit Type t w : seq nat.
 
-  Fixpoint insert (l : nat) (t : seq nat) : seq nat :=
+  Fixpoint insert (t : seq nat) (l : nat) : seq nat :=
     if t is l0 :: t then
       if l < l0 then l :: t
-      else l0 :: (insert l t)
+      else l0 :: (insert t l)
     else [:: l].
 
-  Fixpoint insert_pos (l : nat) (t : seq nat) : nat :=
+  Fixpoint insert_pos (t : seq nat) (l : nat) : nat :=
     if t is l0 :: t then
       if l < l0 then 0
-      else (insert_pos l t).+1
+      else (insert_pos t l).+1
     else 0.
 
 
-  Lemma insert_head_lt l t : head 0 (insert l t) <= l.
+  Lemma insert_head_lt t l : head 0 (insert t l) <= l.
   Proof. case: t => [//=|t0 t] /=; by case (ltnP l t0). Qed.
 
-  Lemma insert_pos_size (l : nat) (t : seq nat) : insert_pos l t <= size t.
+  Lemma insert_pos_size t l : insert_pos t l <= size t.
   Proof. elim: t => //= t0 t; by case (ltnP l t0). Qed.
 
-  Lemma insert_lt_pos (l : nat) (t : seq nat) i :
-    i < (insert_pos l t) -> nth 0 (insert l t) i = nth 0 t i.
+  Lemma insert_lt_pos t l i :
+    i < (insert_pos t l) -> nth 0 (insert t l) i = nth 0 t i.
   Proof.
     elim: t i => //= t0 t; case (ltnP l t0) => //= _ IH.
     case => [_  //=| i Hi] /=; by apply IH.
   Qed.
 
-  Lemma insert_gt_pos (l : nat) (t : seq nat) i :
-    (insert_pos l t) < i -> nth 0 (insert l t) i = nth 0 t i.
+  Lemma insert_gt_pos t l i :
+    (insert_pos t l) < i -> nth 0 (insert t l) i = nth 0 t i.
   Proof.
     elim: t i => [[|n _] //=| t0 t] /=; first by rewrite nth_nil.
     case (ltnP l t0) => Ht H [|i Hi] //=; by apply H.
   Qed.
 
-  Lemma insert_eq_pos (l : nat) (t : seq nat) :
-    nth 0 (insert l t) (insert_pos l t) = l.
+  Lemma insert_eq_pos t l :
+    nth 0 (insert t l) (insert_pos t l) = l.
   Proof.
     elim: t => [//=| t0 t /=]; by case (ltnP l t0).
   Qed.
 
-  Lemma insert_set (l : nat) (t : seq nat) : insert l t = set_nth 0 t (insert_pos l t) l.
+  Lemma insert_set t l : insert t l = set_nth 0 t (insert_pos t l) l.
   Proof.
     elim: t => [//=|t0 t IHt] /=; case (ltnP l t0) => H //=.
     by rewrite IHt.
   Qed.
 
-  Lemma insert_size_non_0 l t : 0 < size (insert l t).
+  Lemma insert_non_nil t l : insert t l != [::].
+  Proof. case: t => [//=|t0 t] /=; case (ltnP l t0) => H //=. Qed.
+
+  Lemma insert_size_non_0 t l : 0 < size (insert t l).
   Proof.
     rewrite insert_set size_set_nth.
-    apply (leq_trans (n := (insert_pos l t).+1)) => //=; by apply leq_maxl.
+    apply (leq_trans (n := (insert_pos t l).+1)) => //=; by apply leq_maxl.
   Qed.
 
-  Lemma insert_pos_lt (l : nat) (t : seq nat) i : i < insert_pos l t -> nth 0 t i <= l.
+  Lemma insert_pos_lt t l i : i < insert_pos t l -> nth 0 t i <= l.
   Proof.
     elim: t i => [//=|t0 t IHt] /=; case (ltnP l t0) => //= Ht.
     case=> [//=|i] /=; by apply IHt.
   Qed.
 
-  Lemma insert_pos_gt (l : nat) (t : seq nat) : l < nth l.+1 t (insert_pos l t).
+  Lemma insert_pos_gt t l : l < nth l.+1 t (insert_pos t l).
   Proof.
     elim: t => [//=|t0 t IHt] /=; by case (ltnP l t0).
   Qed.
 
-  Lemma insert_size_inf l t : (size t) <= size (insert l t).
+  Lemma insert_size_inf t l : (size t) <= size (insert t l).
   Proof.
     elim: t => //= t0 t; by case (ltnP l t0) => //=.
   Qed.
 
-  Lemma insert_size_sup l t : size (insert l t) <= (size t).+1.
+  Lemma insert_size_sup t l : size (insert t l) <= (size t).+1.
   Proof.
     elim: t => //= t0 t; by case (ltnP l t0) => //=.
   Qed.
 
-  Lemma insert_leq l (t : seq nat) : forall (i : nat), nth 0 (insert l t) i <= nth l t i.
+  Lemma insert_leq t l : forall (i : nat), nth 0 (insert t l) i <= nth l t i.
   Proof.
     elim: t => [| t0 t IHt] i /=.
     rewrite nth_nil; case i => [| n]; first by rewrite nth0 /=.
@@ -171,7 +176,7 @@ Section Schensted.
     - by case i => //=.
   Qed.
 
-  Lemma insert_is_row l t : (is_row t) -> is_row (insert l t).
+  Lemma insert_is_row t l : (is_row t) -> is_row (insert t l).
   Proof.
     elim: t => //= l0 [_ _| l1 t IHt /andP [] Hl0l1 Hrow] /=.
     case (ltnP l l0) => //= -> //=.
@@ -180,21 +185,21 @@ Section Schensted.
       move: {Hl0l1 Hlt} Hrow => /= ->; by rewrite (ltnW Hll1).
     - have:= (IHt Hrow) => {IHt Hrow} /=.
       case (ltnP l l1) => /= _; first by rewrite Hlt.
-      case: (insert l t); by rewrite Hl0l1.
+      case: (insert t l); by rewrite Hl0l1.
   Qed.
 
   Fixpoint Sch_rev (w : seq nat) :=
-    if w is l0 :: w' then insert l0 (Sch_rev w')
+    if w is l0 :: w' then insert (Sch_rev w') l0
     else [::].
   Definition Sch w := Sch_rev (rev w).
 
-  Lemma Sch_rcons l (w : seq nat) : Sch (rcons w l) = insert l (Sch w).
+  Lemma Sch_rcons l (w : seq nat) : Sch (rcons w l) = insert (Sch w) l.
   Proof. by rewrite /Sch rev_rcons /=. Qed.
 
   Lemma Sch_size w : size (Sch w) <= size w.
   Proof.
     elim/last_ind: w => [| w l0 IHw] //=.
-    rewrite Sch_rcons; move : (insert_size_sup l0 (Sch w)) => Hins.
+    rewrite Sch_rcons; move : (insert_size_sup (Sch w) l0) => Hins.
     rewrite size_rcons; by apply (leq_trans Hins).
   Qed.
 
@@ -210,27 +215,27 @@ Section Schensted.
   Proof.
     elim/last_ind: w i => [| w l0 IHw] //= i.
     rewrite Sch_rcons insert_set size_set_nth nth_set_nth /=.
-    case: (altP (i =P (insert_pos l0 (Sch w)))).
+    case: (altP (i =P (insert_pos (Sch w) l0))).
     - case: i => [_ _|i]; first by exists [::]; split => //=; rewrite -cats1 suffix_subseq.
-      move=> Hieq _; have := (insert_pos_size l0 (Sch w)); rewrite -Hieq => Hisz.
+      move=> Hieq _; have := (insert_pos_size (Sch w) l0); rewrite -Hieq => Hisz.
       case: (IHw i Hisz) => {Hisz IHw} s [] Hsubs [] Hrow Hsz.
       exists (rcons s (nth 0 (Sch w) i)); split; last split.
       * rewrite -!cats1; apply cat_subseq => //=; first by rewrite cats1.
         by rewrite (eq_refl l0).
-      * have HH : (i < insert_pos l0 (Sch w)) by rewrite Hieq.
-        have Hlt := (insert_pos_lt _ _ _ HH) => {HH}.
+      * have HH : (i < insert_pos (Sch w) l0) by rewrite Hieq.
+        have Hlt := (insert_pos_lt HH) => {HH}.
         apply is_row_rcons => //=; by rewrite last_rcons.
       * by rewrite size_rcons.
-    - case: (altP (insert_pos l0 (Sch w) =P (size (Sch w)))) => [->|].
+    - case: (altP (insert_pos (Sch w) l0 =P (size (Sch w)))) => [->|].
       rewrite /maxn (_ : _.+1 < _ = false) => [Hneq Hlt1|]; last by elim: (size _).
       have Hlt : (i < size (Sch w)) by rewrite ltn_neqAle Hneq.
       case: (IHw i Hlt) => {Hneq Hlt1 Hlt IHw} s /= [] Hsubs [] Hrow Hsz.
       by exists s; split => //=; apply (subseq_trans Hsubs); apply subseq_rcons.
     - rewrite /maxn => Hneq Hneqi Hmax.
       have Hlt : (i < size (Sch w)).
-      case (ltngtP (insert_pos l0 (Sch w)).+1 (size (Sch w))) => //= HH.
+      case (ltngtP (insert_pos (Sch w) l0).+1 (size (Sch w))) => //= HH.
       * by rewrite HH in Hmax.
-      * suff Heq: insert_pos l0 (Sch w) == size (Sch w) by rewrite Heq in Hneq.
+      * suff Heq: insert_pos (Sch w) l0 == size (Sch w) by rewrite Heq in Hneq.
         apply/eqP/anti_leq/andP; split => //=; by apply insert_pos_size.
       * by rewrite HH if_same in Hmax.
       case (IHw i Hlt) => {Hneq Hneqi Hlt IHw Hmax} s /= [] Hsubs [] Hrow Hsz.
@@ -248,47 +253,47 @@ Section Schensted.
       (* s = wn *)
       split; first by apply insert_size_non_0. by apply insert_head_lt.
       (* s = [s] si wn *)
-    - move: (IHw _ _ (is_row_rconsK _ _ Hrow) Hsubs) => [] Hszlt Hlt {IHw}.
-      move: (is_row_last _ _ Hrow); rewrite last_rcons => Hsiwn.
+    - move: (IHw _ _ (is_row_rconsK Hrow) Hsubs) => [] Hszlt Hlt {IHw}.
+      move: (is_row_last Hrow); rewrite last_rcons => Hsiwn.
       rewrite insert_set size_set_nth nth_set_nth maxnC /maxn /=.
-      have Hrowinswn : is_row (insert wn (Sch w))
+      have Hrowinswn : is_row (insert (Sch w) wn)
         by apply insert_is_row; apply Sch_is_row; apply ltnW.
 
-      case (ltnP (size (Sch w)) (insert_pos wn (Sch w)).+1).
+      case (ltnP (size (Sch w)) (insert_pos (Sch w) wn).+1).
 
       (* Insertion add a new [wn] box *)
       * rewrite size_rcons !ltnS => Hsize_ins.
-        have Heqsize: (insert_pos wn (Sch w) = size (Sch w)) by
+        have Heqsize: (insert_pos (Sch w) wn = size (Sch w)) by
           apply anti_leq; apply/andP; split; first by apply insert_pos_size.
         rewrite Heqsize {Hsize_ins}; split; first by [].
         case: (altP ((size s).+1 =P size (Sch w))) => H; first by [].
-        rewrite -[wn](insert_eq_pos _ (Sch w)).
+        rewrite -[wn](insert_eq_pos (Sch w) _).
         have Hlts: ((size s).+1 < size (Sch w)) by rewrite ltn_neqAle; apply/andP.
         rewrite -Heqsize in Hlts {H Hszlt}.
-        rewrite -(insert_lt_pos wn _ _ Hlts).
+        rewrite -(insert_lt_pos Hlts).
         apply/is_rowP => //=; first by apply ltnW.
         by rewrite insert_set size_set_nth maxnC /maxn Heqsize ltnSn ltnSn.
 
       (* Wn bump a letter *)
-      * case: (altP (size (rcons s si) =P insert_pos wn (Sch w))) => [|Hneq Hlts];
+      * case: (altP (size (rcons s si) =P insert_pos (Sch w) wn)) => [|Hneq Hlts];
                                                                     first by move ->.
-        rewrite -[wn](insert_eq_pos _ (Sch w)).
-        move: (insert_pos_gt wn (Sch w)); rewrite (nth_any _ (Sch w) _ 0); last by [].
+        rewrite -[wn](insert_eq_pos (Sch w) _).
+        move: (insert_pos_gt (Sch w) wn); rewrite (@nth_any _ (Sch w) _ 0); last by [].
         move: (leq_trans Hlt Hsiwn) => Hltwn Hwnpos.
         move: (leq_ltn_trans Hltwn Hwnpos) => {Hltwn Hwnpos} Hltnth.
-        move: (row_lt_by_pos _ _ _ (Sch_is_row w) Hszlt Hlts Hltnth) => {Hltnth} Hltswn.
+        move: (row_lt_by_pos (Sch_is_row w) Hszlt Hlts Hltnth) => {Hltnth} Hltswn.
         rewrite size_rcons; rewrite size_rcons in Hneq.
-        have Hltsi: (size s).+1 < insert_pos wn (Sch w) by rewrite ltn_neqAle Hneq Hltswn.
+        have Hltsi: (size s).+1 < insert_pos (Sch w) wn by rewrite ltn_neqAle Hneq Hltswn.
         split; first by apply (ltn_trans Hltsi).
-        rewrite -(insert_lt_pos _ _ _ Hltsi).
+        rewrite -(insert_lt_pos Hltsi).
         apply/is_rowP => //=; apply (leq_trans Hlts); by apply insert_size_inf.
 
     (* The subsequence doesn't end by wn *)
-    - move: (subseq_rcons_neq _ _ _ _ _ Hsiwn Hsubs) => {Hsiwn Hsubs} Hsubs.
+    - move: (subseq_rcons_neq Hsiwn Hsubs) => {Hsiwn Hsubs} Hsubs.
       move: (IHw _ _ Hrow Hsubs) => {IHw Hrow Hsubs} [] Hsize Hleq; split.
       by apply (leq_trans Hsize); apply (insert_size_inf).
-      have:= (insert_leq wn (Sch w) (size s)) => H1.
-      apply (leq_trans H1); by rewrite (nth_any _ _ _ 0).
+      have:= (insert_leq (Sch w) wn (size s)) => H1.
+      apply (leq_trans H1); by rewrite (@nth_any _ _ _ 0).
   Qed.
 
   Definition rowsubseq s w := is_row s /\ subseq s w.
@@ -298,26 +303,20 @@ Section Schensted.
   Proof.
     rewrite /rowsubseq; move=> [].
     case/lastP: s => [//=| s si] =>  Hrow Hsubs.
-    move: (Sch_leq_last _ _ _ Hrow Hsubs) => [] H _.
+    move: (Sch_leq_last Hrow Hsubs) => [] H _.
     by rewrite size_rcons.
   Qed.
 
   Theorem exist_size_Sch w : exists s : seq nat, rowsubseq_n s w (size (Sch w)).
   Proof.
     rewrite /rowsubseq; case/lastP: w => [| w wn]; first by exists [::].
-    move: (insert_size_non_0 wn (Sch w)); rewrite -Sch_rcons.
+    move: (insert_size_non_0 (Sch w) wn); rewrite -Sch_rcons.
     move H : (size _) => ssch; case: ssch H => [_ //=| n] Hn _.
     move: (ltnSn n); rewrite -{2}Hn => H.
-    elim (Sch_exists _ _ H) => s [] Hsubs [] Hrow Hsize.
+    elim (Sch_exists H) => s [] Hsubs [] Hrow Hsize.
     set ss := (rcons _ _) in Hrow; exists ss; split; first by []; split => //=.
     by rewrite /ss size_rcons.
   Qed.
-
-  Fixpoint insert_bump (l : nat) (t : seq nat) : (seq nat)*(option nat) :=
-    if t is l0 :: t then
-      if l < l0 then (l :: t, Some l0)
-      else let: (tr, lr) := insert_bump l t in (l0::tr, lr)
-    else ([:: l], None).
 
 End Schensted.
 
@@ -326,15 +325,15 @@ Section SubSeq.
   Variable w : seq nat.
 
   Definition PRowSeq :=
-    [fun i : nat => [exists s : SubSeq nat_countType w, (is_row s) && (size s == i)]].
+    [fun i : nat => [exists s : SubSeq w, (is_row s) && (size s == i)]].
 
   Lemma exrow0 : PRowSeq 0.
-  Proof. apply /existsP. by exists (sub_nil _ w). Qed.
+  Proof. apply /existsP. by exists (sub_nil w). Qed.
 
   Lemma max_row_len : forall i : nat, PRowSeq i -> i <= size w.
   Proof. rewrite /PRowSeq=> i /= /existsP [[s Hs]] /andP [] _ /eqP <-; by apply size_le. Qed.
 
-  Definition max_rowsubseq_size := ex_maxn (P := PRowSeq) (ex_intro _ 0 exrow0) max_row_len.
+  Definition max_rowsubseq_size := ex_maxn (ex_intro _ 0 exrow0) max_row_len.
 
   Theorem size_max_rowsubseq : max_rowsubseq_size == size (Sch w).
   Proof.
@@ -344,13 +343,338 @@ Section SubSeq.
     rewrite -(eqP Hsz).
     apply/eqP/anti_leq/andP; split.
     - apply size_ndec_Sch; rewrite /rowsubseq; split; first exact Hrow.
-      by apply Hs.
+      rewrite subseqs_all; by apply Hs.
     - rewrite (eqP Hsz); case (exist_size_Sch w) => smax {Hrow Hsz}.
-      rewrite /rowsubseq /rowsubseq_n => [] [] Hrow [] Hsubs /eqP <-.
-      apply Hmax; apply /existsP.
-      exists (exist (is_subseq _ w) smax Hsubs).
+      rewrite /rowsubseq /rowsubseq_n => [] [] Hrow [] /subseqs_all Hsubs /eqP <-.
+      apply Hmax; apply /existsP; exists (SeqSub Hsubs).
       by rewrite Hrow /=.
   Qed.
 
 End SubSeq.
 
+Section Bump.
+
+  Implicit Type l : nat.
+  Implicit Type r w : seq nat.
+  Implicit Type t : seq (seq nat).
+
+  Fixpoint insert_bump r l : (option nat) * (seq nat):=
+    if r is l0 :: r then
+      if l < l0 then (Some l0, l :: r)
+      else let: (lr, rr) := insert_bump r l in (lr, l0 :: rr)
+    else (None, [:: l]).
+
+  Lemma insert_eq_bump r l: (insert_bump r l).2 = insert r l.
+  Proof.
+    elim: r => [//= | t0 r IHt /=].
+    case (ltnP l t0) => _ //=.
+    by move: IHt; case (insert_bump r l) => [lr tr] /= ->.
+  Qed.
+
+  Lemma insert_bump_append r l tr:
+    insert_bump r l = (None, tr) -> tr = rcons r l.
+  Proof.
+    elim: r tr => [[/eqP | a l0 [] <- <-] //=| t0 r IHt ] //=.
+    case (ltnP l t0) => _ //=.
+    move: IHt; case (insert_bump r l) => [[ll //=|]] l0 H tr [] <-.
+    by rewrite (H l0 _).
+  Qed.
+
+  Lemma insert_append_pos r l tr:
+    insert_bump r l = (None, tr) -> (insert_pos r l) = size r.
+  Proof.
+    elim: r tr => [//= | t0 r IHt /=].
+    case (ltnP l t0) => _ //=.
+    move: IHt; case (insert_bump r l) => [[ll //=|] l0 IHt _ _ ].
+    by rewrite (IHt l0).
+  Qed.
+
+  Lemma insert_bump_lt r l ll tr:
+    insert_bump r l = (Some ll, tr) -> l < ll.
+  Proof.
+    elim: r ll tr => [//= | t0 r IHt /=].
+    case (ltnP l t0) => Hcomp /=; first by move => ll tr [] <- _.
+    move: IHt; case (insert_bump r l) => [[lc //=|_ ll tr //=] trr] /= IHt ll tr [] Hlc Htr.
+    subst lc; subst tr; by apply (IHt _ trr).
+  Qed.
+
+  Lemma insert_bump_bump r l ll tr:
+    insert_bump r l = (Some ll, tr) -> ll = (nth 0 r (insert_pos r l)).
+  Proof.
+    elim: r ll tr => [//= | t0 r IHt /=].
+    case (ltnP l t0) => _ /=; first by move => ll tr [] -> _.
+    move: IHt; case (insert_bump r l) => [[lc //=|_ ll tr //=] trr] /= IHt ll tr [] Hlc Htr.
+    subst lc; subst tr; by apply (IHt _ trr).
+  Qed.
+
+  Lemma insert_bump_pos r l ll tr:
+    insert_bump r l = (Some ll, tr) -> (insert_pos r l) < size r.
+  Proof.
+    elim: r ll tr => [//= | t0 r IHt /=].
+    case (ltnP l t0) => _ /=; first by move => ll tr [] _ _.
+    move: IHt; case (insert_bump r l) => [[lc //=|_ _ _ //=] tr] /= IHt _ _ _.
+    by apply (IHt lc tr).
+  Qed.
+
+  Lemma insert_bump_size r l:
+    let: (lr, tr) := insert_bump r l in
+    (size r).+1 == (size tr) + if lr is Some _ then 1 else 0.
+  Proof.
+    elim: r => [//= | t0 r IHt /=].
+    case (ltnP l t0) => _ /=; first by rewrite -addn1.
+    by move: IHt; case (insert_bump r l) => [lr tr] /= /eqP ->.
+  Qed.
+
+  Lemma insert_bump_mult r l i :
+    let: (lr, tr) := insert_bump r l in
+    count_mem i r + (l == i) == count_mem i tr + if lr is Some ll then (ll == i) else 0.
+  Proof.
+    elim: r => [| t0 r IHt] /=; first by rewrite !addn0.
+    case (ltnP l t0) => _ /=.
+    - by rewrite addnC -addnA eqn_add2l addnC eqn_add2l [t0 == i]eq_sym.
+    - move: IHt; case (insert_bump r l) => [tr lr] /= IHt.
+      by rewrite -!addnA eqn_add2l.
+  Qed.
+
+  Fixpoint bump t l : seq (seq nat) :=
+    if t is t0 :: t then
+      let: (lr, tr) := insert_bump t0 l in
+      if lr is Some ll then tr :: (bump t ll) else tr :: t
+    else [:: [:: l]].
+
+  Lemma bump0old t l : nth [::] (bump t l) 0 == insert (nth [::] t 0) l.
+  Proof.
+    case: t => [//=| t0 t /=].
+    rewrite -insert_eq_bump.
+    by case (insert_bump t0 l) => [[ll|] tr].
+  Qed.
+
+  Lemma bump0 (t0 : seq nat) t l b0 b : bump (t0 :: t) l = b0 :: b -> b0 = insert t0 l.
+  Proof.
+    rewrite -insert_eq_bump /=.
+    by case (insert_bump t0 l) => [[l'|]] b' /= [] -> _.
+  Qed.
+
+End Bump.
+
+Section Tableaux.
+
+  Implicit Type l : nat.
+  Implicit Type r u v w : seq nat.
+  Implicit Type t : seq (seq nat).
+
+  Definition dominate u v :=
+    ((size u) <= (size v)) &&
+    [forall i : ordinal (size u), nth 0 u i > nth 0 v i].
+
+  Lemma dominateP u v :
+    reflect ((size u) <= (size v) /\ forall i, i < size u -> nth 0 u i > nth 0 v i)
+            (dominate u v).
+  Proof.
+    rewrite /dominate.
+    apply: (iffP idP).
+    - move=> /andP [] Hsz /forallP Hall; split => [//=| i Hi].
+      by apply (Hall (Ordinal Hi)).
+    - move=> [] -> /= H; apply /forallP => [[i Hi]] /=; by apply H.
+  Qed.
+
+  Lemma dominate_rcons v u l : dominate u v -> dominate u (rcons v l).
+  Proof.
+    move /dominateP => [] Hsz Hlt.
+    apply /dominateP; split => [|i Hi]; first by rewrite size_rcons; apply leqW.
+    move: (Hlt _ Hi) => H.
+    rewrite nth_rcons; case (ltnP i (size v)) => Hcomp //= {H}.
+    move: {Hsz Hlt Hcomp} (leq_trans Hsz Hcomp) => Hs.
+    move: (leq_ltn_trans Hs Hi); by rewrite ltnn.
+  Qed.
+
+  Fixpoint is_tableau t :=
+    match t with
+      | [::] => true
+      | [:: t0] => (t0 != [::]) && is_row t0
+      | t0 :: ((t1 :: _) as ttl) => is_row t0 && dominate t1 t0 && is_tableau ttl
+    end.
+
+  Lemma tableau_is_row r t : is_tableau (r :: t) -> is_row r.
+  Proof. by case t => [| l0 l1 /andP []] /andP [] //=. Qed.
+
+  Lemma tableau_tail r t : is_tableau (r :: t) -> is_tableau t.
+  Proof. by case t => [| l0 l1 /andP []] /andP [] //=. Qed.
+
+  Lemma bump_dominate r1 r0 l tr0 l0:
+    is_row r0 -> is_row r1 -> dominate r1 r0 ->
+    insert_bump r0 l = (Some l0, tr0) -> dominate (insert r1 l0) tr0.
+  Proof.
+    move=> Hrow0 Hrow1 /dominateP [] Hsz Hdom Hins0.
+    apply /dominateP; split.
+    - have := (insert_bump_size r0 l); rewrite Hins0 addn1 => /eqP [] <-.
+      case (ltnP (size r1) (size r0)) => Hcomp;
+          first by apply (leq_trans (insert_size_sup r1 l0)).
+      have: ((size r1) == (size r0)) by rewrite eqn_leq; apply /andP.
+      move=> /eqP Heqsz {Hsz Hcomp}; rewrite -Heqsz.
+      have:= (insert_bump_size r1 l0).
+      move Hins1 : (insert_bump r1 l0) => res1.
+      case: res1 Hins1 => [[l1 |] tr1 Hins1] /=;
+        first by rewrite -insert_eq_bump addn1 Hins1 => /eqP [] ->.
+      (* absurd case:  l0 <= last r0 < last r1  and last r1 <= l0 *)
+      move: (insert_bump_append Hins1) => bla _; subst tr1.
+      have Hins1': (rcons r1 l0) = (insert r1 l0) by rewrite -insert_eq_bump Hins1.
+      have: (is_row (rcons r1 l0)) by rewrite Hins1' insert_is_row.
+
+      move Hsz: (size r0) => n. (* n := size r0 <> 0 *)
+      case: n Hsz => [/eqP /nilP Hnil _| n Hn]; first by move: Hins0; rewrite Hnil.
+
+      move/is_row_last; rewrite -nth_last Heqsz Hn /= => H1.
+
+      have Hnlt : (n < size r1) by rewrite -Hn Heqsz.
+      move: (Hdom _ Hnlt) => /= H2.
+      move: (insert_bump_bump Hins0) => Hl0.
+      move: (insert_bump_pos Hins0); rewrite Hn ltnS => Hpos.
+      move: Hnlt; rewrite Heqsz => Hnlt.
+      move: (is_rowP _ Hrow0 _ _ Hpos Hnlt); rewrite -Hl0 => H3.
+      move: (leq_ltn_trans H1 (leq_ltn_trans H3 H2)); by rewrite ltnn.
+
+    - move=> i Hi.
+      have Hins0': tr0 = (insert r0 l) by rewrite -insert_eq_bump Hins0.
+      rewrite Hins0' !insert_set !nth_set_nth /=.
+      case: (altP (i =P (insert_pos r0 l))) => Hipos0;
+         case: (altP (i =P (insert_pos r1 l0))) => Hipos1.
+      * by apply (insert_bump_lt Hins0).
+      * have Hl: (l <= nth 0 r0 i).
+        - rewrite -(insert_eq_pos r0 l) -Hipos0 -[nth _ r0 _](nth_any l 0);
+              first by apply insert_leq.
+          by rewrite Hipos0 (insert_bump_pos Hins0).
+        apply (leq_ltn_trans Hl).
+        (* LEMMA *)
+        apply Hdom; have:= (insert_bump_size r1 l0).
+        move Hins1 : (insert_bump r1 l0) => res1.
+        case: res1 Hins1 Hi => [[l1 |] tr1 Hins1] /=;
+           first by rewrite -insert_eq_bump addn1 Hins1 /= => Hi /eqP [] ->.
+        case (ltnP i (size r1)) => //= Hi1 Hi2 Htr1.
+        (* absurd case *)
+        have: (i == size r1); move: (leq_trans Hi2 (insert_size_sup r1 l0));
+          first by rewrite ltnS eqn_leq Hi1 => ->.
+        move=> _ {Hi1 Hi2} HH.
+        move: (insert_append_pos Hins1) HH Hipos1 => <- /eqP ->.
+        by rewrite eq_refl.
+      * apply (leq_ltn_trans (n := l)); last by apply (insert_bump_lt Hins0).
+        apply insert_pos_lt.
+        set j := (insert_pos r0 l).
+        case (ltngtP i j) => //= Habs; last by move: Hipos0; rewrite Habs /j eq_refl.
+        (* absurd case *)
+        move: (insert_pos_size r1 l0); rewrite -Hipos1 => H1.
+        move: (leq_trans Habs H1) => H2; move: (Hdom _ H2) => {Hdom H2}.
+        rewrite {1}/j -(insert_bump_bump Hins0) => H2.
+        move: Habs; rewrite Hipos1 => Habs.
+        move: (leq_trans H2 (insert_pos_lt Habs)).
+        by rewrite ltnn.
+      * (* LEMMA *)
+        apply Hdom; have:= (insert_bump_size r1 l0).
+        move Hins1 : (insert_bump r1 l0) => res1.
+        case: res1 Hins1 Hi => [[l1 |] tr1 Hins1] /=;
+           first by rewrite -insert_eq_bump addn1 Hins1 /= => Hi /eqP [] ->.
+        case (ltnP i (size r1)) => //= Hi1 Hi2 Htr1.
+        (* absurd case *)
+        have: (i == size r1); move: (leq_trans Hi2 (insert_size_sup r1 l0));
+          first by rewrite ltnS eqn_leq Hi1 => ->.
+        move=> _ {Hi1 Hi2} HH.
+        move: (insert_append_pos Hins1) HH Hipos1 => <- /eqP ->.
+        by rewrite eq_refl.
+  Qed.
+
+  Lemma bump_tableau t l : is_tableau t -> is_tableau (bump t l).
+  Proof.
+    elim: t l => [l _ //=| t0 t IHt] l Htab /=.
+    move H : (insert_bump t0 l) => x; case: x H => [lr tr].
+    case: lr => [ll |] Hbump.
+    - move: (insert_bump_bump Hbump) => Hll /=.
+      move: {IHt} (IHt ll (tableau_tail Htab)).
+      move Hbp : (bump t ll) => bp.
+      have HH : (tr = insert t0 l) by rewrite -insert_eq_bump Hbump.
+      have Hrowinst0 := (insert_is_row _ (tableau_is_row Htab)).
+      case: bp Hbp => [_| b0 btl Hbp Htabb].
+      * by rewrite HH Hrowinst0 insert_non_nil.
+      * rewrite Htabb {1}HH Hrowinst0 /= andbT.
+        case: t Htab Hbp => [Htab /= [] <- _| t1 t Htabt01 Hbump1].
+        * have H : ([:: ll] = insert [::] ll) by [].
+          have Hdom : (dominate [::] t0) by
+             rewrite /dominate /=; apply /forallP => [[m /=]]; rewrite ltn0.
+          rewrite H; apply (bump_dominate (r0 := t0) (l := l)) => //=.
+          by move: Htab => /= /andP [] _.
+        * have Htabt1 := (tableau_is_row (tableau_tail Htabt01)).
+          move: Htabt01 => /= /andP [] /andP [] Htabt0 Hdom _.
+          rewrite (bump0 Hbump1).
+          by apply (bump_dominate Htabt0 Htabt1 Hdom Hbump).
+    - move: (insert_bump_append Hbump) => HH {IHt}; subst tr.
+      have HH : (rcons t0 l = insert t0 l) by rewrite -insert_eq_bump Hbump.
+      case: t Htab (tableau_tail Htab) => [/= /andP [] Htab Hnnil _| t1 t].
+      * rewrite rcons_non_nil /= HH; by apply insert_is_row.
+      * move=> /= /andP [] /andP [] Hrowt0 Hdom -> _.
+        apply /andP; split; last by []; apply /andP; split;
+            first by rewrite HH; by apply insert_is_row.
+        by apply dominate_rcons.
+  Qed.
+
+  Definition to_word t := flatten (rev t).
+
+  Fixpoint RS_rev w : seq (seq nat) :=
+    if w is w0 :: wr then
+      bump (RS_rev wr) w0
+    else [::].
+  Definition RS w := RS_rev (rev w).
+
+  Theorem RS_tableau w : is_tableau (RS w).
+  Proof.
+    elim/last_ind: w => [//=| w l0].
+    rewrite /RS rev_rcons /=.
+    by apply bump_tableau.
+  Qed.
+
+End Tableaux.
+
+(*
+Eval compute in (RS [:: 2; 5; 1; 6; 4; 3]).
+Eval compute in (to_word (RS [:: 2; 5; 1; 6; 4; 3])).
+*)
+
+(*
+
+  Fixpoint bump_row_rev r w : (seq nat) * (seq nat) :=
+    if w is w0 :: wr then
+      let: (remw, tres) := bump_row_rev r wr in
+      let: (lr, rr) := (insert_bump tres w0) in
+      if lr is Some ll then (rcons remw ll, rr) else (remw, rr)
+    else ([::], r).
+  Definition bump_row r w := bump_row_rev r (rev w).
+
+  Lemma count_mem_rcons w l i : count_mem i (rcons w l) = count_mem i w + (l == i).
+  Proof. by rewrite -count_rev rev_rcons /= count_rev addnC. Qed.
+
+  Lemma bump_size r w :
+    let: (remw, tres) := bump_row r w in
+    size r + size w == size remw +  size tres.
+  Proof.
+    rewrite/bump_row.
+    elim/last_ind: w => [| w l0] /=; first by rewrite addnC.
+    rewrite rev_rcons /=.
+    case (bump_row_rev r (rev w)) => [remw tres].
+    rewrite size_rcons addnS => /eqP ->; rewrite -addnS.
+    have:= insert_bump_size tres l0.
+    case (insert_bump tres l0) => [[ll|] tr] /eqP ->; last by rewrite addn0.
+    by rewrite size_rcons addnA addSn addn1.
+  Qed.
+
+  Lemma bump_mult r w i :
+    let: (remw, tres) := bump_row r w in
+    count_mem i r + count_mem i w == count_mem i remw + count_mem i tres.
+  Proof.
+    rewrite/bump_row.
+    elim/last_ind: w => [| w l0] /=; first by rewrite addnC.
+    rewrite rev_rcons /=.
+    case (bump_row_rev r (rev w)) => [remw tres].
+    rewrite count_mem_rcons addnA=> /eqP ->.
+    rewrite -addnA; have:= insert_bump_mult tres l0 i.
+    case (insert_bump tres l0) => [[ll|] tr] /eqP ->; last by rewrite addn0.
+    by rewrite count_mem_rcons -addnA eqn_add2l addnC.
+  Qed.
+*)        
