LRrule/subseq.v
@@ -1,5 +1,8 @@
 Require Import ssreflect ssrbool ssrfun ssrnat eqtype choice fintype seq.
 
+Set Implicit Arguments.
+Unset Strict Implicit.
+
 Section RCons.
 
   Variable (T : eqType).
@@ -48,107 +51,59 @@ Section RCons.
 End RCons.
 
 Section Fintype.
+  (* We define SubSeq w as a finType *)
 
   Variable (T : countType).
   Implicit Type s w : seq T.
   Implicit Type a b l : T.
 
-  Fixpoint subseqs_dup w :=
+  Fixpoint subseqs w :=
     if w is w0 :: w' then
-      [seq w0 :: s | s <- subseqs_dup w' ] ++ subseqs_dup w'
+      [seq w0 :: s | s <- subseqs w' ] ++ subseqs w'
     else [:: [::] ].
-
-  Definition subseqs w := undup (subseqs_dup w).
 
   Lemma subseqs_all s w : subseq s w <-> s \in subseqs w.
   Proof.
-    rewrite mem_undup; split.
-    elim: w s => [H /eqP -> //=| w0 w IHw].
-    have Hinjcons: injective (cons w0) by move=> x1 x2 [].
-    case=> [_|s0 s]; simpl; first by rewrite mem_cat (IHw _ (sub0seq w)); apply orbT.
-    case: (altP (s0 =P w0)) => [-> | _] H; move: {H} (IHw _ H); rewrite mem_cat.
-    - by rewrite -[s \in _](mem_map Hinjcons) => ->.
-    - by move->; apply orbT.
-    elim: w s => [H | w0 w IHw]; first by rewrite mem_seq1.
-    have Hinjcons: injective (cons w0) by move=> x1 x2 [].
-    case=> [_|s0 s /=]; first by apply sub0seq.
-    case: (altP (s0 =P w0)) => [->|Hneq]; rewrite mem_cat => /orP [].
-    * rewrite (mem_map Hinjcons); by apply IHw.
-    * move/IHw => H; by apply (subseq_trans (subseq_cons _ _) H).
-    * move/cons_in_map_cons => H; rewrite (eqP (H s)) in Hneq.
-      by rewrite (eq_refl w0) in Hneq.
-    * by apply IHw.
+    split; elim: w s => [H| w0 w IHw].
+    * by move=> /eqP ->.
+    * have Hinjcons: injective (cons w0) by move=> x1 x2 [].
+      case=> [_|s0 s]; simpl; first by rewrite mem_cat (IHw _ (sub0seq w)); apply orbT.
+      case: (altP (s0 =P w0)) => [-> | _] H; move: {H} (IHw _ H); rewrite mem_cat.
+      - by rewrite -[s \in _](mem_map Hinjcons) => ->.
+      - by move->; apply orbT.
+
+    * by rewrite mem_seq1.
+    * have Hinjcons: injective (cons w0) by move=> x1 x2 [].
+      case=> [_|s0 s /=]; first by apply sub0seq.
+      case: (altP (s0 =P w0)) => [->|Hneq]; rewrite mem_cat => /orP [].
+      - rewrite (mem_map Hinjcons); by apply IHw.
+      - move/IHw => H; by apply (subseq_trans (subseq_cons _ _) H).
+      - move/cons_in_map_cons => H; rewrite (eqP (H s)) in Hneq.
+        by rewrite (eq_refl w0) in Hneq.
+      - by apply IHw.
   Qed.
 
-  Definition is_subseq w := fun s => subseq s w.
+  Definition SubSeq w := seq_sub (subseqs w).
+  Coercion seq_of_SubSeq w (s : (SubSeq w)) : seq T := ssval s.
 
-  Definition SubSeq w := {s | is_subseq w s}.
+  Definition Sub_of_subseq w s : subseq s w -> SubSeq w.
+  Proof. move => H; apply (SeqSub (ssval := s)); by rewrite -subseqs_all. Defined.
 
-  Definition sub_eqMixin w := sig_eqMixin (is_subseq w).
-  Canonical sub_eqType w := sig_eqType (is_subseq w).
-
-  Definition sub_nil w : (SubSeq w) :=
-    (exist (is_subseq w) [::] (sub0seq (T := T) w)).
-
-  Definition sub_full w : (SubSeq w) :=
-    (exist (is_subseq w) w (subseq_refl w)).
-
-  Definition sub_extend (w0 : T) w (s : SubSeq w) : SubSeq (w0 :: w).
-  case: s => s Ps; exists s; apply (subseq_trans Ps); by apply subseq_cons. Defined.
-
-  Lemma sub_extend_eq (w0 : T) w : val \o (sub_extend w0 w) =1 val.
-  Proof. by case=> s Ps /=. Qed.
-
-  Definition sub_cons (w0 : T) w (s : SubSeq w) : SubSeq (w0 :: w).
-  case: s => s Ps; exists (w0 :: s); by rewrite /= (eq_refl w0). Defined.
-
-  Lemma sub_cons_eq (w0 : T) w : [eta val] \o [eta sub_cons w0 w] =1 (cons w0) \o val.
-  Proof. by case=> s Ps /=. Qed.
-
-  Fixpoint SubSeqs_dup w : seq (SubSeq w) :=
-    match w as w return seq (SubSeq w) with
-      | [::] => [:: sub_nil [::]]
-      | w0 :: w =>
-        [seq sub_cons  w0 w s | s <- SubSeqs_dup w ] ++
-        [seq sub_extend w0 w s | s <- SubSeqs_dup w ]
-    end.
-  Definition SubSeqs w := undup (SubSeqs_dup w).
-
-  Lemma val_SubSeqs w : subseqs_dup w == [seq val s | s <- SubSeqs_dup w].
-  Proof.
-    elim: w => [//=|w0 w IHw /=].
-    rewrite map_cat -!map_comp (eq_map (sub_cons_eq w0 w)) (eq_map (sub_extend_eq w0 w)).
-    by rewrite (eqP IHw) -map_comp.
-  Qed.
-
-  Lemma mem_val_SubSeqs w (s : (SubSeq w)) :
-    (s \in SubSeqs_dup w) = (val s \in subseqs_dup w).
-  Proof. rewrite (eqP (val_SubSeqs w)) mem_map //=; by apply val_inj. Qed.
-
-  Lemma SubSeqs_enumP w : Finite.axiom (SubSeqs w).
-  Proof.
-    rewrite /Finite.axiom /SubSeqs => S.
-    rewrite count_uniq_mem; last by apply undup_uniq.
-    rewrite mem_undup mem_val_SubSeqs /= -mem_undup.
-    case: S => s /=; rewrite subseqs_all; by move ->.
-  Qed.
-
-  Definition SubSeq_finMixin w := Eval hnf in FinMixin (SubSeqs_enumP w).
-  Canonical SubSeq_finType w := Eval hnf in FinType (SubSeq w) (SubSeq_finMixin w).
-  Coercion seq_of_SubSeq w (s : (SubSeq w)) := val s.
+  Definition sub_nil  w : (SubSeq w) := Sub_of_subseq (sub0seq w).
+  Definition sub_full w : (SubSeq w) := Sub_of_subseq (subseq_refl w).
 
   Lemma size_le w (s : (SubSeq w)) : size s <= size w.
-  Proof. case: s => s Ps; by apply size_subseq. Qed.
+  Proof. case: s => s Ps /=; apply size_subseq; by rewrite subseqs_all. Qed.
 
 End Fintype.
 
-Section MaxLen.
+Section MaxSize.
 
   Variable w : seq nat.
-  Definition PSeq := [fun i : nat => [exists s : SubSeq nat_countType w, size s == i]].
+  Definition PSeq := [fun i : nat => [exists s : SubSeq w, size s == i]].
 
   Lemma ex0 : PSeq 0.
-  Proof. apply /existsP. by exists (sub_nil _ w). Qed.
+  Proof. apply /existsP. by exists (sub_nil w). Qed.
 
   Lemma max_len : forall i : nat, PSeq i -> i <= size w.
   Proof. rewrite /PSeq => i /= /existsP [[s Hs]] /eqP <-; by apply size_le. Qed.
@@ -161,8 +116,8 @@ Section MaxLen.
     apply/eqP/anti_leq/andP; split; first by apply max_len.
     suff: PSeq (size w); first by apply Hleqi.
     rewrite /PSeq /=; apply /existsP.
-    by exists (sub_full _ w).
+    by exists (sub_full  w).
   Qed.
 
-End MaxLen.
+End MaxSize.
 
